lean/Nucleus/Nucleus/Hol/Ethane.lean
@@ -10,7 +10,6 @@ import Nucleus.Hol.Ethane.FV
 import Nucleus.Hol.Ethane.Builtin
 import Nucleus.Hol.Ethane.LogicalOpcode
 import Nucleus.Hol.Ethane.ClassicalMatrix
-import Nucleus.Hol.Ethane.ClassicalSequent
 import Nucleus.Hol.Ethane.Arena
 import Nucleus.Hol.Ethane.Arena.Cbor
 import Nucleus.Hol.Ethane.Arena.OneBased
